WIP

theories/Template/QuoteGround/Coq/ssr.v
@@ -1,28 +1,23 @@
 From MetaCoq.Lob.Template.QuoteGround Require Export Coq.Init.
-From Coq.ssr Require Import ssrbool.
+From Coq.ssr Require Import ssrbool ssreflect.
 
 #[export] Instance quote_if_spec {A b vT vF} {not_b:Prop} {b' a} {qA : quotation_of A} {qvT : quotation_of vT} {qvF : quotation_of vF} {qnot_b : quotation_of not_b} {quote_not_b : ground_quotable not_b} : ground_quotable (@if_spec A b vT vF not_b b' a) := ltac:(destruct 1; exact _).
-Print alt_spec.
-#[export] Instance quote_if_spec {A b vT vF} {not_b:Prop} {b' a} {qA : quotation_of A} {qvT : quotation_of vT} {qvF : quotation_of vF} {qnot_b : quotation_of not_b} {quote_not_b : ground_quotable not_b} : ground_quotable (@if_spec A b vT vF not_b b' a) := ltac:(destruct 1; exact _).
-Variant alt_spec : bool -> Type :=
-Variant implies P Q := Implies of P -> Q.
-Inductive and3 (P1 P2 P3 : Prop) : Prop := And3 of P1 & P2 & P3.
-Inductive and4 (P1 P2 P3 P4 : Prop) : Prop := And4 of P1 & P2 & P3 & P4.
-Inductive and5 (P1 P2 P3 P4 P5 : Prop) : Prop :=
+#[export] Instance quote_alt_spec {P:Prop} {b b'} {qP : quotation_of P} {quoteP : ground_quotable P} : ground_quotable (@alt_spec P b b') := ltac:(destruct 1; exact _).
+Section and.
+  Context {P1 P2 P3 P4 P5 : Prop}
+          {qP1 : quotation_of P1} {qP2 : quotation_of P2} {qP3 : quotation_of P3} {qP4 : quotation_of P4} {qP5 : quotation_of P5}
+          {quoteP1 : ground_quotable P1} {quoteP2 : ground_quotable P2} {quoteP3 : ground_quotable P3} {quoteP4 : ground_quotable P4} {quoteP5 : ground_quotable P5}.
+
+  #[export] Instance quote_and3 : ground_quotable (and3 P1 P2 P3) := (ltac:(destruct 1; exact _)).
+  #[export] Instance quote_and4 : ground_quotable (and4 P1 P2 P3 P4) := (ltac:(destruct 1; exact _)).
+  #[export] Instance quote_and5 : ground_quotable (and5 P1 P2 P3 P4 P5) := (ltac:(destruct 1; exact _)).
+End and.
+#[export] Existing Instances quote_and3 quote_and4 quote_and5.
+(* can't do or without decidability *)
+(*
 Inductive or3 (P1 P2 P3 : Prop) : Prop := Or31 of P1 | Or32 of P2 | Or33 of P3.
 Inductive or4 (P1 P2 P3 P4 : Prop) : Prop :=
-(** Variant of simpl_pred specialised to the membership operator. **)
-Variant mem_pred T := Mem of pred T.
-Variant qualifier (q : nat) T := Qualifier of {pred T}.
-Variant pred_key (p : {pred T}) : Prop := DefaultPredKey.
-Inductive external_view : Type := tactic_view of Type.
-Variant put vT sT (v1 v2 : vT) (s : sT) : Prop := Put.
-  Inductive indt_type (p : p_str) := Indt ... .
-Variant phantom T (p : T) : Prop := Phantom.
-Variant phant (p : Type) : Prop := Phant.
- construction of dependent Records and Structures. For example, if we need
-    Record r := R {x; y : T(x)}.
-Variant simpl_fun (aT rT : Type) := SimplFun of aT -> rT.
-Variant bijective : Prop := Bijective g of cancel f g & cancel g f.
-
-Locate and4.
+ *)
+#[export] Instance quote_put {vT sT v1 v2 s} {qvT : quotation_of vT} {qsT : quotation_of sT} {qv1 : quotation_of v1} {qv2 : quotation_of v2} {qs : quotation_of s} : ground_quotable (@TheCanonical.put vT sT v1 v2 s) := ltac:(destruct 1; exact _).
+#[export] Instance quote_phantom {T p} {qT : quotation_of T} {qp : quotation_of p} : ground_quotable (@phantom T p) := ltac:(destruct 1; exact _).
+#[export] Instance quote_phant {p} {qp : quotation_of p} : ground_quotable (@phant p) := ltac:(destruct 1; exact _).
