theories/Template/QuoteGround/utils/MCList.v
@@ -1,0 +1,4 @@
+From MetaCoq.Lob.Template.QuoteGround Require Export Coq.Init.
+From MetaCoq.Template.utils Require Import MCList.
+
+#[export] Instance quote_nth_error_Spec {A l n o} {qA : quotation_of A} {quoteA : ground_quotable A} {qo : quotation_of o} {ql : quotation_of l} : ground_quotable (@nth_error_Spec A l n o) := ltac:(destruct 1; exact _).
