theories/Template/QuoteGround/utils/MCOption.v
@@ -1,0 +1,20 @@
+From MetaCoq.Lob.Template.QuoteGround Require Export Coq.Init.
+From MetaCoq.Template.utils Require Import MCOption.
+
+#[local] Hint Extern 0 => reflexivity : typeclass_instances.
+
+#[export] Instance quote_ForOption {A P o} {qA : quotation_of A} {qP : quotation_of P} {qo : quotation_of o} {quoteP : forall t, o = Some t -> ground_quotable (P t:Prop)} : ground_quotable (@ForOption A P o).
+Proof.
+  destruct o; adjust_ground_quotable_by_econstructor_inversion (); eauto.
+Defined.
+
+#[export] Instance quote_option_extends {A o1 o2} {qA : quotation_of A} {qo1 : quotation_of o1} {qo2 : quotation_of o2} {quoteA : forall t, o2 = Some t -> quotation_of t} : ground_quotable (@option_extends A o1 o2).
+Proof.
+  destruct o1 as [a|], o2 as [a'|].
+  all: try specialize (quoteA _ eq_refl).
+  all: try solve [ intro pf; exfalso; inversion pf ].
+  all: try (intro pf; assert (a = a') by (now inversion pf); subst;
+            let t := type of pf in
+            revert pf; change (ground_quotable t)).
+  all: adjust_ground_quotable_by_econstructor_inversion ().
+Defined.
