theories/Template/QuoteGround/utils/MCReflect.v
@@ -1,0 +1,4 @@
+From MetaCoq.Lob.Template.QuoteGround Require Export Coq.Init.
+From MetaCoq.Template.utils Require Import MCReflect.
+
+#[export] Instance quote_reflectT {A} {qA : quotation_of A} {quoteA : ground_quotable A} {quote_negA : ground_quotable (A -> False)} {b} : ground_quotable (@reflectT A b) := ltac:(destruct 1; exact _).
